Quicksort/Partition/BentleyMcIlroy/Basic.lean
@@ -12,15 +12,15 @@ private def move_pivots_back (left right : Nat) (hlr : left < right) (hr : right
     (p q : Nat) (hp : p < n) (x : { x : Partition α n // left < x.i' ∧ x.j' < right ∧ x.i' ≤ q + 1 }) :
     { x : Partition α n // left < x.i' ∧ x.j' < right } :=
   let ⟨⟨arr', j', i'⟩, (_ : left < i'), (_ : j' < right), (_ : i' ≤ q + 1)⟩ := x
-  let rec move_p_back (k : Nat) (arr : Vector α n) (j : Nat) (hjr : j < right) (_ : j < right) :
+  let rec @[specialize] move_p_back (k : Nat) (arr : Vector α n) (j : Nat) (hjr : j < right) :
       Vector α n × Subtype (· < right) :=
     if h : k < p then
-      move_p_back (k + 1) (arr.swap k j (by omega) (by omega)) (j - 1) (by omega)  (by omega)
+      move_p_back (k + 1) (arr.swap k j (by omega) (by omega)) (j - 1) (by omega)
     else
       (arr, ⟨j, by omega⟩)
-  let (arr'', ⟨j'', _⟩) := move_p_back (left + 1) arr' j' (by omega)  (by omega)
+  let (arr'', ⟨j'', _⟩) := move_p_back (left + 1) arr' j' (by omega)
 
-  let rec move_q_forward (k : Nat) (arr : Vector α n) (i : Nat) (hkq : q + 1 ≤ k) (hli : left < i)
+  let rec @[specialize] move_q_forward (k : Nat) (arr : Vector α n) (i : Nat) (hkq : q + 1 ≤ k) (hli : left < i)
       (hieqk_invar : i = k - (q + 1) + i') : Vector α n × Subtype (left < ·) :=
 
     if h : k < right then
@@ -116,8 +116,6 @@ def eager (arr : Vector α n) (left : Nat) (right : Nat)
 
 
 namespace classic
-variable (lt_asymm : ∀ {x y : α}, lt x y → ¬lt y x)
-variable (le_trans : ∀ {x y z : α}, ¬lt y x → ¬lt z y → ¬lt z x)
 
 @[inline]
 private def loop.while_j' (left right : Nat) (hr : right < n) (hl : left < n) (pivot : α)
@@ -144,10 +142,14 @@ private def loop.while_i'  (left right : Nat) (hr : right < n) (pivot : α) (arr
   else
     ⟨⟨ival, by omega⟩, hii, hxi, h'⟩
 
+section
+open Ord in
 @[inline]
-def _root_.Partition.bentleyMcIlroy.classic (arr : Vector α n) (left : Nat) (right : Nat)
+def _root_.Partition.bentleyMcIlroy.classic  [inst_le_trans : Std.TransOrd α] (arr : Vector α n) (left : Nat) (right : Nat)
     (hlr : left < right) (hr : right < n)
     : { x : Partition α n  // left < x.i' ∧ x.j' < right } :=
+  have lt_asymm : ∀ {x y : α}, lt x y → ¬lt y x := by grind
+  have le_trans' : ∀ {x y z : α}, ¬lt y x → ¬lt z y → ¬lt z x := by grind
   have hl : left < n := by omega
   let mid := left + ((right - left)/2)
   have hm : mid < n := by omega
@@ -158,7 +160,7 @@ def _root_.Partition.bentleyMcIlroy.classic (arr : Vector α n) (left : Nat) (ri
   let pivot := arr_[mid]
 
   have : ¬lt pivot arr_[left] ∧ ¬lt arr_[right] pivot :=
-    median_of_three_sorted lt_asymm le_trans (by omega) (by omega) hr
+    median_of_three_sorted (by omega) (by omega) hr
 
   -- let arr_ := dbg arr_ s!"arr1: {arr_},  left: {left}, right: {right}, i': {i_}, j': {j_}, p: {p_}, q: {q_}"
   have hrr : right - 1 + 1 = right := by omega
@@ -268,20 +270,20 @@ where
         else
           ⟨⟨arr, j' - 1, i' + 1⟩, by simp only; omega, by simp only; omega, by simp only; omega⟩
   -- termination_by j + 1 - i
-
+end
 
 
 /-- info: { arr' := { toArray := #[4, 3, 1, 0, 5, 2, 6, 8, 7, 9], size_toArray := _ }, j' := 5, i' := 7 } -/
-#guard_msgs(info) in #eval! Partition.bentleyMcIlroy.classic sorry sorry #v[9,  3,  1,  8,  6,  2,  5,  0,  7,  4]  0 9 (by omega) (by omega)
+#guard_msgs(info) in #eval Partition.bentleyMcIlroy.classic #v[9,  3,  1,  8,  6,  2,  5,  0,  7,  4]  0 9 (by omega) (by omega)
 
 /-- info: { arr' := { toArray := #[4, 2, 1, 0, 3, 6, 6, 8, 7, 9], size_toArray := _ }, j' := 4, i' := 7 } -/
-#guard_msgs(info) in #eval! Partition.bentleyMcIlroy.classic sorry sorry #v[9,  3,  1,  8,  6,  2,  6,  0,  7,  4]  0 9 (by omega) (by omega)
+#guard_msgs(info) in #eval Partition.bentleyMcIlroy.classic #v[9,  3,  1,  8,  6,  2,  6,  0,  7,  4]  0 9 (by omega) (by omega)
 
 /-- info: { arr' := { toArray := #[4, 2, 1, 0, 3, 6, 6, 8, 7, 9], size_toArray := _ }, j' := 4, i' := 7 } -/
-#guard_msgs(info) in #eval! Partition.bentleyMcIlroy.classic sorry sorry #v[9,  3,  1,  8,  6,  2,  6,  0,  7,  4]  0 9 (by omega) (by omega)
+#guard_msgs(info) in #eval Partition.bentleyMcIlroy.classic #v[9,  3,  1,  8,  6,  2,  6,  0,  7,  4]  0 9 (by omega) (by omega)
 
 /-- info: { arr' := { toArray := #[0, 0, 0, 1, 2], size_toArray := _ }, j' := 0, i' := 3 } -/
-#guard_msgs(info) in #eval! Partition.bentleyMcIlroy.classic sorry sorry #v[2, 0, 0, 1, 0]  0 4 (by omega) (by omega)
+#guard_msgs(info) in #eval Partition.bentleyMcIlroy.classic #v[2, 0, 0, 1, 0]  0 4 (by omega) (by omega)
 
 -- end
 end  classic
@@ -310,148 +312,3 @@ def Partition.bentleyMcIlroy [Ord α] (arr : Vector α n) (left : Nat)  (right :
       (by omega) (by omega) (by omega) (by omega) (by omega) (by omega)
     |> (Inhabited.mk ·)
     panic! "non-asymmetric or non-transitive comparitor. falling back to eager version of hoare partition scheme"
-
-
-
-  -- @[specialize] move_pivots_back (p q : Nat) (x : { x : Partition α n  // left < x.i' ∧ x.j' < right })  :
-  --     { x : Partition α n  // left < x.i' ∧ x.j' < right } := Id.run do
-  --   let mut ⟨⟨arr', j', i'⟩, (_ : left < i'), (_ : j' < right)⟩ := x
-  --   ---
-  --   for _' : k in [left + 1 : p] do
-  --     arr' := arr'.swap k j' sorry sorry
-  --     j' := j' - 1
-
-
-  --   for _' : k in [q + 1 : right] do
-  --     arr' := arr'.swap k i' (by sorry) (by sorry)
-  --     i' := i' + 1
-  --   ---
-  --   return ⟨⟨arr', j', i'⟩, by sorry, by sorry⟩
-
-
-
-
-
-
-  -- have : ¬ lt arr[i'] pivot ∨ j < i' (lt pivot arr[i'] ∨ (¬ lt arr[i'] pivot ∧ ¬ lt pivot arr[i']))
-  -- have : arr[i'] ≥ pivot ∨ i' > j'
-
-  -- ¬ lt arr[i'] < pivot
-  -- lt arr[i'] < pivot ∨ lt pivot < arr[i']
-  -- show i' > j' → arr[i'] > pivot
-  -- show i' = j' → arr[i'+1] > pivot
-
-
-
-  -- ¬ lt pivot arr[j'] ∨ i ≤ j' (lt arr[j'] pivot ∨ (¬ lt pivot arr[j'] ∧ ¬ lt arr[j'] pivot) )
-
-
-
-
-
-
-      -- ----
-      -- let arr' := arr.swap i' j' (by omega) (by omega)
-      -- let (arr₂, ⟨p', (_ : p' ≤ p + 1)⟩) : Vector α n × Subtype (· ≤ p + 1) :=
-      --   if h : ¬ lt arr'[i'] pivot then
-      --     (arr'.swap p i' (by omega) (by omega), ⟨p + 1, by solve_by_elim⟩)
-      --   else
-      --     (arr', ⟨p, by solve_by_elim⟩)
-
-      -- let (arr'', ⟨q', (_ : q' < right)⟩) : Vector α n × Subtype (· < right) :=
-      --   if h : ¬ lt pivot arr₂[j'] then
-      --     (arr₂.swap q j' (by omega) (by omega), ⟨q - 1, by omega⟩)
-      --   else
-      --     (arr₂, ⟨q, by solve_by_elim⟩)
-      -- ---
-      -- have  : RangeHas n (fun i_ => ¬lt arr''[i_] pivot = true ∧ ¬lt pivot arr''[i_] = true) (q' + 1) right := by sorry
-      -- -- exact
-      -- loop pivot arr'' (i' + 1) (j' - 1) p' q' (by omega)  (by omega)  (by omega) (by omega) (by omega) this
-
-
-
-
-
-
-
-
--- open Vector
--- attribute [grind →] Membership.mem.upper
--- @[inline]
--- def Partition.bentleyMcIlroy [Inhabited α] /- [ToString α] -/ [Ord α] {n : Nat}
---     (arr : Vector α n) (left : Nat)  (right : Nat) (hlr : left < right) (hr : right < n) :
---     {x : Partition α n // (left < x.i') ∧ (x.j' < right)} := Id.run do
-
---   let mid := left + (right - left) / 2
-
---   let mut arr := arr
---     |> (maybeSwap · ⟨left, sorry⟩ ⟨mid, sorry⟩)
---     |> (maybeSwap · ⟨left, sorry⟩ ⟨right, sorry⟩)
---     |> (maybeSwap · ⟨mid, sorry⟩ ⟨right, sorry⟩)
-
---   let pivot := arr[mid]
-
-
---   let mut i := left + 1
---   let mut j := right - 1
-
---   let mut p := left + 1
---   let mut q := right - 1
-
---   -- arr := dbg arr s!"arr1: {arr},  left: {left}, right: {right}, i: {i}, j: {j}, p: {p}, q: {q}"
---   while true do
-
---     while /- i ≠ right ∧ -/ lt arr[i]! pivot do
---       i := i + 1
-
-
---     while /- left ≠ j ∧ -/ lt pivot arr[j]! do
---       j := j - 1
-
---     if i < j then
---       arr := arr.swap i j sorry sorry
-
---       if ¬ lt arr[i]! pivot then
---         arr := arr.swap p i sorry sorry
---         p := p + 1
-
---       if ¬ lt pivot arr[j]! then
---         arr := arr.swap q j sorry sorry
---         q := q - 1
-
---       i := i + 1
---       j := j - 1
---       continue
---     else
-
-
---       if j < i then
---         break
---       else
---         i := i + 1
---         j := j - 1
-
---         break
-
---   -- arr := dbg arr s!"arr3: {arr},  left: {left}, right: {right}, i: {i}, j: {j}, p: {p}, q: {q}"
---   for k in [left + 1 : p] do
---     arr := arr.swap k j sorry sorry
---     j := j - 1
-
-
---   for k in [q + 1 : right] do
---     arr := arr.swap k i sorry sorry
---     i := i + 1
-
---   return ⟨⟨arr, j, i⟩, by sorry, by sorry⟩
-
-
-
-
-
-
-
--- #eval! Partition.bentleyMcIlroy #v[9,  3,  1,  8,  6,  2,  5,  0,  7,  4]  0 9 (by omega) (by omega)
--- #eval! Partition.bentleyMcIlroy #v[9,  3,  1,  8,  6,  2,  6,  0,  7,  4]  0 9 (by omega) (by omega)
--- #eval! Partition.bentleyMcIlroy #v[9,  3,  1,  8,  6,  2,  6,  0,  7,  4]  0 9 (by omega) (by omega)
--- #eval! Partition.bentleyMcIlroy #v[2, 0, 0, 1, 0]  0 4 (by omega) (by omega)
