Quicksort/Partition/Lemmas.lean
@@ -8,28 +8,16 @@ open Vector
 namespace Partition
 variable [Ord α]
 
--- private class LT_Asymm (α : Type u) [Ord α] : Prop where
--- private class LE_Trans (α : Type u) [Ord α] : Prop where
-
--- -- variable (le_trans : ∀ {x y z : α}, ¬lt y x → ¬lt z y → ¬lt z x)
--- -- variable (lt_asymm : ∀ {x y : α}, lt x y → ¬lt y x)
-
-class StrictOrder (α : Type u) [Ord α]  : Prop where
-  lt_asymm : ∀ {x y : α}, lt x y → ¬lt y x
-  le_trans : ∀ {x y z : α}, ¬lt y x → ¬lt z y → ¬lt z x
-
-export StrictOrder (lt_asymm le_trans)
-
-
 class LawfulScheme (part : Partition.Scheme α) : Prop where
   partitionBounds : (part as left right hlr hr).val.j' < (part as left right hlr hr).val.i'
   permStabilizing : PermStabilizing' left right (part as left right hlr hr).val.arr' as
-  sorting [StrictOrder α] (as : Vector α n) (hlr : left < right) (hr : right < n) : ∃ (pivot : α), IsPartitioned left right pivot (part as left right hlr hr).val
+  sorting [Std.TransOrd α] (as : Vector α n) (hlr : left < right) (hr : right < n) : ∃ (pivot : α), IsPartitioned left right pivot (part as left right hlr hr).val
 
+open Ord
 instance instLawfulHoareScheme : LawfulScheme (α := α) hoare where
   partitionBounds := hoare.partition_bounds
   permStabilizing := hoare.permStabilizing
-  sorting _ _ _ := hoare.sorted lt_asymm le_trans
+  sorting _ _ _ := hoare.sorted
 
 instance instLawfulLomutoScheme : LawfulScheme (α := α) lomuto where
   partitionBounds := lomuto.partition_bounds
