Quicksort/Init/Ord.lean
@@ -1,0 +1,98 @@
+module
+variable [Ord α]
+
+namespace Std
+
+
+@[simp]
+public theorem not_lt_iff_eq_swap :
+    (∀ {x y : α}, ¬(compare y x |>.isLT) ↔ (compare x y |>.isLE)) ↔
+    (∀ {x y : α}, compare x y = (compare y x).swap) := by
+  constructor
+  · intro not_lt
+    intro x y
+    have _ := not_lt (x := x) (y := y)
+    have _ := not_lt (x := y) (y := x)
+    cases h : compare x y <;> cases _ : compare y x <;>
+      simp_all
+
+  · intro eq_swap
+    intro x y
+    cases h : compare y x <;> simp [h, eq_swap]
+
+@[grind =]
+public theorem eq_swap_of_not_lt :
+    (∀ {x y : α}, ¬(compare y x |>.isLT) ↔ (compare x y |>.isLE)) →
+    (∀ {x y : α}, compare x y = (compare y x).swap) := not_lt_iff_eq_swap.1
+
+
+@[simp, grind .]
+public theorem OrientedOrd.isLE_iff_not_LT [OrientedOrd α] : ∀ {x y : α}, ¬(compare y x |>.isLT) ↔  (compare x y |>.isLE) :=
+  not_lt_iff_eq_swap.2 OrientedOrd.eq_swap
+
+@[grind ·]
+public theorem OrientedOrd.isLT_asymm' (eq_swap : ∀ {x y : α}, compare x y = (compare y x).swap) : ∀ {x y : α}, (compare x y).isLT → ¬(compare y x).isLT := by
+  intro x y
+  cases h :  compare x y <;> simp [h, eq_swap]
+
+
+
+
+@[grind ·]
+public theorem OrientedOrd.isLT_asymm [OrientedOrd α] : ∀ {x y : α}, (compare x y).isLT → ¬(compare y x).isLT := by
+  intro x y
+  have _ : compare y x = (compare x y).swap := OrientedOrd.eq_swap
+  cases _ :  compare x y <;> simp_all
+
+
+
+
+
+public instance instTransOrdOfnot_lt_le_trans
+    (not_lt : ∀ {x y : α}, ¬(compare y x |>.isLT) ↔ (compare x y |>.isLE) := by grind)
+    (le_trans : ∀ {x y z : α}, (compare x y).isLE → (compare y z).isLE → (compare x z).isLE := by grind) :
+    TransOrd α where
+  isLE_trans := le_trans
+  eq_swap := not_lt_iff_eq_swap.1 not_lt
+
+
+
+attribute [grind .] TransOrd.isLE_trans
+
+@[grind ·]
+public theorem TransOrd.isLE_trans' [TransOrd α] :
+    ∀ {x y z : α}, ¬(compare y x |>.isLT) → ¬(compare z y |>.isLT) → ¬(compare z x |>.isLT) := by
+  grind
+
+end Std
+
+
+@[expose, inline]
+public abbrev lt (x y : α) := compare x y |>.isLT
+@[expose, inline]
+public abbrev le (x y : α) := compare x y |>.isLE
+
+
+
+namespace Ord
+open Std
+-- aliases of the above
+public theorem not_lt [OrientedOrd α] : ∀ {x y : α}, ¬lt y x ↔ le x y := OrientedOrd.isLE_iff_not_LT
+public theorem le_trans [TransOrd α] : ∀ {x y z : α}, le x y → le y z → le x z := TransOrd.isLE_trans
+public theorem lt_asymm [OrientedOrd α] : ∀ {x y : α}, lt x y → ¬lt y x := OrientedOrd.isLT_asymm
+public theorem le_trans' [TransOrd α] : ∀ {x y z : α}, ¬lt y x → ¬lt z y → ¬lt z x := TransOrd.isLE_trans'
+
+end Ord
+public theorem Ord.lt_irrefl (lt_asymm : ∀ {x y : α}, lt x y → ¬lt y x) : ∀ (x : α), ¬lt x x := fun _ h => (lt_asymm h) h
+
+
+
+namespace examples
+private scoped instance : Ord (Bool × String) := lexOrd
+example : ∀ {x y z : Bool × String}, le x y → le y z → le x z := by grind
+example : ∀ {x y : UInt32}, lt x y → ¬lt y x := by grind
+example : ∀ {x y z : UInt32}, ¬lt y x → ¬lt z y → ¬lt z x := by grind
+
+example : ∀ {x y : Int}, lt x y → ¬lt y x := by grind
+example : ∀ {x y z : Int}, ¬lt y x → ¬lt z y → ¬lt z x := by grind
+end examples
