Quicksort/Partition/Lomuto/Lemmas.lean
@@ -5,11 +5,6 @@ open Vector
 
 namespace Partition
 variable [Ord α]
-variable (lt_asymm : ∀ {x y : α}, lt x y → ¬lt y x)
-
-include lt_asymm in
-private theorem lt_irrefl : ∀ (x : α), ¬lt x x :=
-  fun _ h => (lt_asymm h) h
 
 protected theorem lomuto.loop.partition_bounds {left right : Nat}  {hlr : left < right} {hr : right < n} {pivot : α} {arr : Vector α n} {i j : Nat} {hli : left ≤ i} {hij : i ≤ j} {hjr : j ≤ right} : (loop left right hlr hr pivot arr i j hli hij hjr).val.j' < (loop left right hlr hr pivot arr i j hli hij hjr).val.i' := by
   induction arr, i, j, hli, hij, hjr using lomuto.loop.induct (hr := hr) (pivot := pivot)  with
@@ -176,8 +171,10 @@ protected theorem lomuto.loop.sorted {left right : Nat} {hlr : left < right} {hr
         grind only [getElem_swap]
 
 
-variable (le_trans : ∀ {x y z : α}, ¬lt y x → ¬lt z y → ¬lt z x)
+-- variable [Std.OrientedOrd α]
+variable (lt_asymm : ∀ {x y : α}, lt x y → ¬lt y x)
 
+open Ord in
 include lt_asymm in
 protected theorem lomuto.sorted {arr : Vector α n} {left : Nat} {right : Nat} {hlr : left < right} {hr : right < n} : ∃ (pivot : α), IsPartitioned left right pivot (lomuto arr left right hlr hr).val := by
   let mid := left + ((right - left)/2)
