SortExperiments/Adapt.lean
@@ -1,0 +1,29 @@
+
+import Quicksort.Partition.Basic
+import SortExperiments.InsertionSort
+
+
+
+
+@[inline]
+def qs_adapt [Ord α] (arr : Array α) (left : Nat := 0) (right : Nat := arr.size - 1) (M := 0) (part : Partition.Scheme α := @default _ _) : Array α :=
+  -- let part := @Partition.dutch α
+  let rec @[specialize]
+  strict {n : Nat} (as : Vector α n) (left : Nat := 0) (right : Nat := n - 1) (hsize' : right ≤ n - 1) : Vector α n :=
+    if hlr : left + M < right then
+      let ⟨⟨as', j', i'⟩, (_ : _ < i'), (_ : j' < _ )⟩ := part as left right (by omega) (by omega)
+      let as := qs_adapt.strict as' left j' (by omega)
+      let as := qs_adapt.strict as i' right (by omega)
+      as
+    else
+      as.insertionSort left right
+    termination_by right - left
+
+  let right' : Nat := if right ≤ arr.size - 1 then right else
+    have := Inhabited.mk (arr.size - 1)
+    panic! "index out of bounds"
+
+  have : right' ≤ arr.size - 1 := by
+    simp [right']; split <;> simp [panicWithPosWithDecl, panic, panicCore, *]
+
+  qs_adapt.strict ⟨arr, rfl⟩ left right' this |>.1
