SortExperiments/PDQSort.lean
@@ -1,0 +1,229 @@
+
+import Quicksort.Basic
+import Quicksort.Partition.BentleyMcIlroy.Basic
+import SortExperiments.HeapSort
+-- import SortExperiments.Adapt
+import SortExperiments.InsertionSort
+
+
+@[inline]
+public def pdqsort1 [Ord α] (arr : Array α) (left : Nat := 0) (right : Nat := arr.size - 1) (M := 0) : Array α :=
+  let rec
+    @[specialize]
+    strict {n : Nat} (as : Vector α n) (_left : Nat := 0) (_right : Nat := n - 1) (hsize' : _right ≤ n - 1)
+        (allowed_bad_partitions : Nat := n.log2)
+        (parent_pivot : Option α := none) : Vector α n :=
+
+      let len := _right - _left + 1
+
+      if hlr : M + 1 < len then
+        if allowed_bad_partitions > 0 then
+
+          have hl : _left < n := by omega
+          have hr : _right < n := by omega
+          let mid := _left + ((_right - _left)/2)
+          have hm : mid < n := by omega
+          let as_ := as
+            |> (Vector.maybeSwap · ⟨_left, hl⟩ ⟨mid, hm⟩)
+            |> (Vector.maybeSwap · ⟨_left, hl⟩ ⟨_right, hr⟩)
+            |> (Vector.maybeSwap · ⟨mid, hm⟩ ⟨_right, hr⟩)
+          let pivot := as_[mid]
+
+          let is_duplicate_run : Bool :=
+            match parent_pivot with
+            | some p => compare pivot p == .eq
+            | none => false
+
+
+          let ⟨⟨as', j', i'⟩, (_ : _left < i'), (_ : j' < _right )⟩ :=
+            if is_duplicate_run then
+              Partition.bentleyMcIlroy.classic.loop _left _right (by omega) (by omega) pivot as_
+                (i := _left + 1)
+                (j := _right - 1)
+                (p := _left + 1)
+                (q := _right - 1)
+                (by omega) (by omega) (by omega) (by omega)  (by omega) (by omega) sorry sorry
+            else
+              Partition.hoare.classic.loop _left _right (by omega) (by omega) pivot as_
+                (_left + 1)
+                (_right - 1)
+                (by omega) (by omega) (by omega) sorry sorry
+
+          let left_len := (j' - _left) + 1
+          let right_len := (_right - i') + 1
+
+          let unbalanced := !is_duplicate_run && (left_len < (len / 8) || right_len < (len / 8))
+
+          let next_bad_left := if unbalanced then allowed_bad_partitions - 1 else allowed_bad_partitions
+          let next_bad_right := if unbalanced then allowed_bad_partitions - 1 else allowed_bad_partitions
+
+          let as''' :=
+            if left_len < right_len then
+              let as'' := strict as' _left j' (by omega) next_bad_left none
+              strict as'' i' _right (by omega) next_bad_right (some pivot)
+            else
+              let as'' := strict as' i' _right (by omega) next_bad_right (some pivot)
+              strict as'' _left j' (by omega) next_bad_left none
+
+          as'''
+
+        else
+          as.heapSort _left _right (by omega) (by omega)
+      else
+        as.insertionSort _left _right
+      termination_by _right - _left
+
+
+  let right' : Nat := if right ≤ arr.size - 1 then right else
+    have := Inhabited.mk (arr.size - 1)
+    panic! "index out of bounds"
+
+  have : right' ≤ arr.size - 1 := by
+    simp [right']; split <;> simp [panicWithPosWithDecl, panic, panicCore, *]
+
+  strict ⟨arr, rfl⟩ left right' this arr.size.log2 none  |>.1
+
+def test_array := #[
+  56, 69, 30, 11, 34, 14, 95, 81, 96, 76,
+  91, 24, 13, 39, 42, 14, 46, 3, 4, 61,
+  84, 68, 58, 39, 95, 85, 34, 29, 47, 3,
+  40, 8, 91, 60, 43, 88, 25, 39, 35, 89,
+  5, 37, 90, 94, 86, 53, 43, 39, 14, 29,
+  10, 91, 77, 24, 32, 99, 7, 3, 37, 73,
+  63, 0, 30, 57, 93, 79, 27, 1, 17, 53,
+  4, 0, 6, 65, 16, 18, 70, 54, 90, 41,
+  42, 78, 52, 50, 49, -0, 19, 40, 33, 26,
+  84, 75, 99, 4, 91, 50, 53, 60, 56, 24
+]
+
+-- def expected_array := #[
+--   -0, 0, 0, 1, 3, 3, 3, 4, 4, 4, 5, 6, 7,
+--   8, 10, 11, 13, 14, 14, 14, 16, 17, 18, 19,
+--   24, 24, 24, 25, 26, 27, 29, 29, 30, 30, 32,
+--   33, 34, 34, 35, 37, 37, 39, 39, 39, 39, 40,
+--   40, 41, 42, 42, 43, 43, 46, 47, 49, 50, 50,
+--   52, 53, 53, 53, 54, 56, 56, 57, 58, 60, 60,
+--   61, 63, 65, 68, 69, 70, 73, 75, 76, 77, 78,
+--   79, 81, 84, 84, 85, 86, 88, 89, 90, 90, 91,
+--   91, 91, 91, 93, 94, 95, 95, 96, 99, 99
+-- ]
+
+
+/--
+info: #[0, 0, 0, 1, 3, 3, 3, 4, 4, 4, 5, 6, 7, 8, 10, 11, 13, 14, 14, 14, 16, 17, 18, 19, 24, 24, 24, 25, 26, 27, 29, 29, 30,
+  30, 32, 33, 34, 34, 35, 37, 37, 39, 39, 39, 39, 40, 40, 41, 42, 42, 43, 43, 46, 47, 49, 50, 50, 52, 53, 53, 53, 54,
+  56, 56, 57, 58, 60, 60, 61, 63, 65, 68, 69, 70, 73, 75, 76, 77, 78, 79, 81, 84, 84, 85, 86, 88, 89, 90, 90, 91, 91,
+  91, 91, 93, 94, 95, 95, 96, 99, 99]
+-/
+#guard_msgs in
+#eval! pdqsort1 (M := 34) test_array
+
+
+-- @[inline]
+-- private def filter_equals [Ord α] (pivot : α) (arr : Vector α n) (left right : Nat) (hr : right < n) : Vector α n × Subtype (left < ·) :=
+--   let rec
+--     @[specialize]
+--     loop (arr : Vector α n) (i eq_end : Nat) (hir : eq_end ≤ i) (h_progress : left < eq_end) :=
+--       if hir : i ≤ right then
+--         have _ : i < n := by omega
+--         if _ : compare arr[i] pivot = .eq then
+--           let arr' := arr.swap i eq_end (by omega) (by omega)
+--           loop arr' (i + 1) (eq_end + 1) (by omega) (by omega)
+--         else
+--           loop arr (i + 1) eq_end (by omega) (by omega)
+--       else
+--         (arr, ⟨eq_end, h_progress⟩)
+--   loop arr (left + 1) (left + 1) (by omega) (by omega)
+
+
+@[inline]
+public def pdqsort2 [Ord α] (arr : Array α) (left : Nat := 0) (right : Nat := arr.size - 1) (M := 0)  : Array α :=
+  let rec
+    @[specialize]
+    strict {n : Nat} (as : Vector α n) (left : Nat := 0) (right : Nat := n - 1) (hsize' : right ≤ n - 1 := by omega)
+        -- (allowed_bad_partitions : Nat := n.log2)
+        -- (parent_pivot : Option α := none)
+        : Vector α n :=
+
+      let len := right - left + 1
+
+      -- have _ : _left + M < _right ↔ M + 1 < len := by omega
+      have hl : left < n := by sorry
+      have hr : right < n := by omega
+      let mid := left + ((right - left)/2)
+
+      -- have _ :  left + ((right - left)/2) =  left + (len/2) := by grind
+      have hm : mid < n := by omega
+      let as_ := as
+        |> (Vector.maybeSwap · ⟨left, hl⟩ ⟨mid, hm⟩)
+        |> (Vector.maybeSwap · ⟨left, hl⟩ ⟨right, hr⟩)
+        |> (Vector.maybeSwap · ⟨mid, hm⟩ ⟨right, hr⟩)
+      if hlr : M + 1 < len then
+        -- if allowed_bad_partitions > 0 then
+
+          let pivot := as_[mid]
+
+          -- let is_duplicate_run : Bool :=
+          --   match parent_pivot with
+          --   | some p => compare pivot p == .eq
+          --   | none => false
+
+
+          -- if !is_duplicate_run then
+            let ⟨⟨as, j', i'⟩, (_ : left < i'), (_ : j' < right )⟩ :=
+                Partition.hoare.classic.loop left right (by omega) (by omega) pivot as_
+                  (left + 1)
+                  (right - 1)
+                  (by omega) (by omega) (by omega) sorry sorry
+
+            -- let left_len := (j' - _left) + 1
+            -- let right_len := (_right - i') + 1
+
+            -- let unbalanced := /- !is_duplicate_run && -/ (left_len < (len / 8) || right_len < (len / 8))
+
+            -- let next_bad_left := if unbalanced then allowed_bad_partitions - 1 else allowed_bad_partitions
+            -- let next_bad_right := if unbalanced then allowed_bad_partitions - 1 else allowed_bad_partitions
+
+
+              let as := strict as left j' (by omega)
+              let as := strict as i' right (by omega)
+              as
+
+
+            -- if left_len < right_len then
+            --   let as'' := strict as' _left j' (by omega) /- next_bad_left -/ /- none -/
+            --   strict as'' i' _right (by omega) /- next_bad_right -/ /- (some pivot) -/
+            -- else
+            --   let as'' := strict as' i' _right (by omega) next_bad_right /- (some pivot) -/
+            --   strict as'' _left j' (by omega) next_bad_left /- none -/
+
+
+          -- else
+          --   let ⟨as', ⟨next_left, _⟩⟩ := filter_equals pivot as_ _left _right (by omega)
+          --   strict as' next_left _right (by omega) (allowed_bad_partitions := allowed_bad_partitions) (parent_pivot := none)
+
+        -- else
+        --   Vector.heapSort as _left _right (by omega) (by omega)
+      else
+        as.insertionSort left right
+      termination_by right - left
+
+
+  let right' : Nat := if right ≤ arr.size - 1 then right else
+    have := Inhabited.mk (arr.size - 1)
+    panic! "index out of bounds"
+
+  have : right' ≤ arr.size - 1 := by
+    simp [right']; split <;> simp [panicWithPosWithDecl, panic, panicCore, *]
+
+  strict ⟨arr, rfl⟩ left right' this /- arr.size.log2 -/ /- none -/  |>.1
+
+
+/--
+info: #[0, 0, 0, 1, 3, 3, 3, 4, 4, 4, 5, 6, 7, 8, 10, 11, 13, 14, 14, 14, 16, 17, 18, 19, 24, 24, 24, 25, 26, 27, 29, 29, 30,
+  30, 32, 33, 34, 34, 35, 37, 37, 39, 39, 39, 39, 40, 40, 41, 42, 42, 43, 43, 46, 47, 49, 50, 50, 52, 53, 53, 53, 54,
+  56, 56, 57, 58, 60, 60, 61, 63, 65, 68, 69, 70, 73, 75, 76, 77, 78, 79, 81, 84, 84, 85, 86, 88, 89, 90, 90, 91, 91,
+  91, 91, 93, 94, 95, 95, 96, 99, 99]
+-/
+#guard_msgs in
+#eval! pdqsort2 (M := 34) test_array
